src/OperationalSem.v
@@ -1,132 +1,163 @@
 Require Import List.
+Import ListNotations.
 Require Import Coq.Lists.ListSet.
-Require Import Unify.
-Require Import MiniKanrenSyntax.
-Require Import Stream.
+Require Import Coq.Program.Equality.
 Require Import Omega.
 Require Import Extraction.
 
-(* Partial state *) 
-Inductive state' : Set :=
-(* (goal, subst, first free semantic variable) *) | Leaf : goal -> subst -> nat -> state'
-(* sum of two states'                          *) | Sum  : state' -> state' -> state'
-(* product of two states'                      *) | Prod : state' -> goal   -> state'.
+Require Import Unify.
+Require Import Stream.
+Require Import MiniKanrenSyntax.
+Require Import DenotationalSem.
 
-(* Complete state *)
+
+(************************* States *************************)
+
+Inductive nt_state : Set :=
+| Leaf : goal -> subst -> nat -> nt_state
+| Sum  : nt_state -> nt_state -> nt_state
+| Prod : nt_state -> goal   -> nt_state.
+
 Inductive state : Set :=
-(* end of evaluation *) | Stop  : state
-(* a partial state   *) | State : state' -> state.
+| Stop  : state
+| NTState : nt_state -> state.
 
-Inductive is_fv_of_state' : name -> state' -> Prop :=
-| isfvst'Leaf  : forall x g s n     (X_FV_G : is_fv_of_goal x g),
-                                    is_fv_of_state' x (Leaf g s n)
-| isfvst'SumL  : forall x st'1 st'2 (X_FV : is_fv_of_state' x st'1),
-                                    is_fv_of_state' x (Sum st'1 st'2)
-| isfvst'SumR  : forall x st'1 st'2 (X_FV : is_fv_of_state' x st'2),
-                                    is_fv_of_state' x (Sum st'1 st'2)
-| isfvst'ProdL : forall x st' g     (X_FV : is_fv_of_state' x st'),
-                                    is_fv_of_state' x (Prod st' g)
-| isfvst'ProdR : forall x st' g     (X_FV : is_fv_of_goal x g),
-                                    is_fv_of_state' x (Prod st' g).
+Inductive is_fv_of_nt_state : name -> nt_state -> Prop :=
+| isfvnstLeaf  : forall x g s n  (X_FV_G : is_fv_of_goal x g),
+                                    is_fv_of_nt_state x (Leaf g s n)
+| isfvnstSumL  : forall x nst1 nst2 (X_FV : is_fv_of_nt_state x nst1),
+                                    is_fv_of_nt_state x (Sum nst1 nst2)
+| isfvnstSumR  : forall x nst1 nst2 (X_FV : is_fv_of_nt_state x nst2),
+                                    is_fv_of_nt_state x (Sum nst1 nst2)
+| isfvnstProdL : forall x nst g     (X_FV : is_fv_of_nt_state x nst),
+                                    is_fv_of_nt_state x (Prod nst g)
+| isfvnstProdR : forall x nst g     (X_FV : is_fv_of_goal x g),
+                                    is_fv_of_nt_state x (Prod nst g).
 
-Hint Constructors is_fv_of_state'.
+Hint Constructors is_fv_of_nt_state : core.
 
 Inductive is_fv_of_state : name -> state -> Prop :=
-| isfvstC : forall x st' (X_FV_ST' : is_fv_of_state' x st'),
-                         is_fv_of_state x (State st').
+| isfvstC : forall x nst (X_FV_NT_ST : is_fv_of_nt_state x nst),
+                         is_fv_of_state x (NTState nst).
 
-Hint Constructors is_fv_of_state.
+Hint Constructors is_fv_of_state : core.
 
-Inductive is_counter_of_state' : nat -> state' -> Prop :=
-| iscst'Leaf  : forall g s n,      is_counter_of_state' n (Leaf g s n)
-| iscst'SumL  : forall n st'1 st'2 (ISC : is_counter_of_state' n st'1),
-                                   is_counter_of_state' n (Sum st'1 st'2)
-| iscst'SumR  : forall n st'1 st'2 (ISC : is_counter_of_state' n st'2),
-                                   is_counter_of_state' n (Sum st'1 st'2)
-| iscst'Prod  : forall n st' g     (ISC : is_counter_of_state' n st'),
-                                   is_counter_of_state' n (Prod st' g).
+Inductive is_counter_of_nt_state : nat -> nt_state -> Prop :=
+| iscnstLeaf  : forall g s n,      is_counter_of_nt_state n (Leaf g s n)
+| iscnstSumL  : forall n nst1 nst2 (ISC : is_counter_of_nt_state n nst1),
+                                   is_counter_of_nt_state n (Sum nst1 nst2)
+| iscnstSumR  : forall n nst1 nst2 (ISC : is_counter_of_nt_state n nst2),
+                                   is_counter_of_nt_state n (Sum nst1 nst2)
+| iscnstProd  : forall n nst g     (ISC : is_counter_of_nt_state n nst),
+                                   is_counter_of_nt_state n (Prod nst g).
 
-Hint Constructors is_counter_of_state'.
+Hint Constructors is_counter_of_nt_state : core.
 
-Inductive well_formed_state' : state' -> Set :=
-| wfLeaf : forall g s frn   (DOM_LT_COUNTER :  forall x (X_IN_DOM : in_subst_dom s x),
-                                                        x < frn)
-                            (VRAN_LT_COUNTER : forall x (X_IN_VRAN : in_subst_vran s x),
-                                                        x < frn)
-                            (FV_LT_COUNTER :   forall x (X_FV : is_fv_of_goal x g),
-                                                        x < frn),
-                            well_formed_state' (Leaf g s frn)
-| wfSum  : forall st'1 st'2 (WF_L : well_formed_state' st'1)
-                            (WF_R : well_formed_state' st'2),
-                            well_formed_state' (Sum st'1 st'2)
-| wfProd : forall st' g     (WF_L : well_formed_state' st')
-                            (FV_LT_COUNTER : forall x frn (FRN_COUNTER : is_counter_of_state' frn st')
+Inductive well_formed_nt_state : nt_state -> Set :=
+| wfLeaf : forall g s frn
+           (DOM_LT_COUNTER  : forall x (X_IN_DOM : in_subst_dom s x), x < frn)
+           (VRAN_LT_COUNTER : forall x (X_IN_VRAN : in_subst_vran s x), x < frn)
+           (FV_LT_COUNTER   : forall x (X_FV : is_fv_of_goal x g), x < frn),
+           well_formed_nt_state (Leaf g s frn)
+| wfSum  : forall nst1 nst2 (WF_L : well_formed_nt_state nst1)
+                            (WF_R : well_formed_nt_state nst2),
+                            well_formed_nt_state (Sum nst1 nst2)
+| wfProd : forall nst g     (WF_L : well_formed_nt_state nst)
+                            (FV_LT_COUNTER : forall x frn (FRN_COUNTER : is_counter_of_nt_state frn nst)
                                                           (X_FV : is_fv_of_goal x g),
                                                           x < frn),
-                            well_formed_state' (Prod st' g).
+                            well_formed_nt_state (Prod nst g).
 
-Hint Constructors well_formed_state'.
+Hint Constructors well_formed_nt_state : core.
+
+Fixpoint first_nats (k : nat) : list nat :=
+  match k with
+  | 0   => []
+  | S n => n :: first_nats n
+  end.
+
+Lemma first_nats_less (n k : nat) (H : In n (first_nats k)) : n < k.
+Proof.
+  induction k.
+  { inversion H. }
+  { inversion H. { omega. } { apply IHk in H0. omega. } }
+Qed.
+
+Lemma well_formed_initial_state
+      (g   : goal)
+      (k   : nat)
+      (HC  : closed_goal_in_context (first_nats k) g) :
+      well_formed_nt_state (Leaf g empty_subst k).
+Proof.
+  constructor.
+  { intros. good_inversion X_IN_DOM. good_inversion H. }
+  { intros. good_inversion X_IN_VRAN. destruct H as [t0 [H0 _]]. good_inversion H0. }
+  { red in HC. intros. apply first_nats_less; auto. }
+Qed.
+
 
 Inductive well_formed_state : state -> Set :=
-| wfEmpty    : well_formed_state Stop
-| wfNonEmpty : forall st' (wfState : well_formed_state' st'),
-                          well_formed_state (State st').
+| wfTerminal    : well_formed_state Stop
+| wfNonTerminal : forall nst (wfState : well_formed_nt_state nst),
+                             well_formed_state (NTState nst).
 
-Hint Constructors well_formed_state.
+Hint Constructors well_formed_state : core.
 
+
+
+(************************** LTS ***************************)
 (* Labels *)
 Inductive label : Set :=
-(* nothing                                       *) | Step   : label
-(* answer: (subst, first free semantic variable) *) | Answer : subst -> nat -> label.
+| Step   : label
+| Answer : subst -> nat -> label.
 
 (* Transitions *)
-Inductive eval_step : state' -> label -> state -> Set :=
-| esFail         : forall           s    n, eval_step (Leaf Fail s n) Step Stop
-| esCut          : forall           s    n, eval_step (Leaf Cut s n)  (Answer s n) Stop                             (* cuts are ignored in interliving search *)
-| esUnifyFail    : forall t1 t2     s    n  (MGU : mgu (apply_subst s t1) (apply_subst s t2) None),
-                                            eval_step (Leaf (Unify t1 t2) s n) Step Stop
-| esUnifySuccess : forall t1 t2     s s' n  (MGU : mgu (apply_subst s t1) (apply_subst s t2) (Some s')),
-                                            eval_step (Leaf (Unify t1 t2) s n) (Answer (compose s s') n) Stop
-| esDisj         : forall g1 g2     s    n, eval_step (Leaf (Disj g1 g2) s n) Step (State (Sum (Leaf g1 s n) (Leaf g2 s n)))
-| esConj         : forall g1 g2     s    n, eval_step (Leaf (Conj g1 g2) s n) Step (State (Prod (Leaf g1 s n) g2))
-| esFresh        : forall fg        s    n, eval_step (Leaf (Fresh fg) s n)   Step (State (Leaf (fg n) s (S n)))
-| esInvoke       : forall r arg     s    n, eval_step (Leaf (Invoke r arg) s n) Step (State (Leaf (proj1_sig (MiniKanrenSyntax.Prog r) arg) s n))
-| esSumE         : forall st1 st2        l  (STEP_L : eval_step st1 l  Stop),
-                                            eval_step (Sum st1 st2) l (State st2)
-| esSumNE        : forall st1 st1' st2   l  (STEP_L : eval_step st1 l (State st1')),
-                                            eval_step (Sum st1 st2) l (State (Sum st2 st1'))
-| esProdSE       : forall st g              (STEP_L : eval_step st Step Stop),
-                                            eval_step (Prod st g) Step Stop
-| esProdAE       : forall st g s n          (STEP_L : eval_step st (Answer s n) Stop),
-                                            eval_step (Prod st g) Step (State (Leaf g s n))
-| esProdSNE      : forall st g     st'      (STEP_L : eval_step st Step (State st')),
-                                            eval_step (Prod st g) Step (State (Prod st' g))
-| esProdANE      : forall st g s n st'      (STEP_L : eval_step st (Answer s n) (State st')),
-                                            eval_step (Prod st g) Step (State (Sum (Leaf g s n) (Prod st' g))).
+Inductive eval_step : nt_state -> label -> state -> Set :=
+| esFail    : forall s n, eval_step (Leaf Fail s n) Step Stop
+| esUnifyFail    : forall t1 t2 s   n (MGU : mgu (apply_subst s t1) (apply_subst s t2) None),
+                                      eval_step (Leaf (Unify t1 t2) s n) Step Stop
+| esUnifySuccess : forall t1 t2 s d n (MGU : mgu (apply_subst s t1) (apply_subst s t2) (Some d)),
+                                      eval_step (Leaf (Unify t1 t2) s n) (Answer (compose s d) n) Stop
+| esDisj         : forall g1 g2 s n, eval_step (Leaf (Disj g1 g2) s n)   Step (NTState (Sum (Leaf g1 s n) (Leaf g2 s n)))
+| esConj         : forall g1 g2 s n, eval_step (Leaf (Conj g1 g2) s n)   Step (NTState (Prod (Leaf g1 s n) g2))
+| esFresh        : forall fg    s n, eval_step (Leaf (Fresh fg) s n)     Step (NTState (Leaf (fg n) s (S n)))
+| esInvoke       : forall r arg s n, eval_step (Leaf (Invoke r arg) s n) Step (NTState (Leaf (proj1_sig (MiniKanrenSyntax.Prog r) arg) s n))
+| esSumE         : forall nst1       nst2 l (STEP_L : eval_step nst1 l  Stop),
+                                            eval_step (Sum nst1 nst2) l (NTState nst2)
+| esSumNE        : forall nst1 nst1' nst2 l (STEP_L : eval_step nst1 l (NTState nst1')),
+                                            eval_step (Sum nst1 nst2) l (NTState (Sum nst2 nst1'))
+| esProdSE       : forall nst g          (STEP_L : eval_step nst Step Stop),
+                                         eval_step (Prod nst g) Step Stop
+| esProdAE       : forall nst g s n      (STEP_L : eval_step nst (Answer s n) Stop),
+                                         eval_step (Prod nst g) Step (NTState (Leaf g s n))
+| esProdSNE      : forall nst g     nst' (STEP_L : eval_step nst Step (NTState nst')),
+                                         eval_step (Prod nst g) Step (NTState (Prod nst' g))
+| esProdANE      : forall nst g s n nst' (STEP_L : eval_step nst (Answer s n) (NTState nst')),
+                                         eval_step (Prod nst g) Step (NTState (Sum (Leaf g s n) (Prod nst' g))).
 
-Hint Constructors eval_step.
+Hint Constructors eval_step : core.
 
 Lemma counter_in_answer
-      (st' : state')
+      (nst : nt_state)
       (s : subst)
       (n : nat)
       (st : state)
-      (EV : eval_step st' (Answer s n) st) :
-      is_counter_of_state' n st'.
+      (EV : eval_step nst (Answer s n) st) :
+      is_counter_of_nt_state n nst.
 Proof.
   remember (Answer s n). induction EV; good_inversion Heql; auto.
 Qed.
 
 Lemma counter_in_next_state
       (n : nat)
-      (st' st'_next : state')
+      (nst nst_next : nt_state)
       (l : label)
-      (EV : eval_step st' l (State st'_next))
-      (ISC_NEXT :  is_counter_of_state' n st'_next) :
-      exists n', n' <= n /\ is_counter_of_state' n' st'.
+      (EV : eval_step nst l (NTState nst_next))
+      (ISC_NEXT :  is_counter_of_nt_state n nst_next) :
+      exists n', n' <= n /\ is_counter_of_nt_state n' nst.
 Proof.
-  remember (State st'_next) as st.
-  revert Heqst ISC_NEXT. revert st'_next.
+  remember (NTState nst_next) as st.
+  revert Heqst ISC_NEXT. revert nst_next.
   induction EV; intros; good_inversion Heqst.
   { exists n. split.
     { constructor. }
@@ -143,7 +174,7 @@ Proof.
   { exists n. split.
     { constructor. }
     { auto. } }
-  { specialize (IHEV st1' eq_refl). good_inversion ISC_NEXT.
+  { specialize (IHEV nst1' eq_refl). good_inversion ISC_NEXT.
     { exists n. split.
       { constructor. }
       { auto. } }
@@ -151,10 +182,10 @@ Proof.
       exists n'; auto. } }
   { good_inversion ISC_NEXT. exists n0.
     eapply counter_in_answer in EV. split; auto. }
-  { specialize (IHEV st' eq_refl). good_inversion ISC_NEXT.
+  { specialize (IHEV nst' eq_refl). good_inversion ISC_NEXT.
     apply IHEV in ISC. destruct ISC as [n' [LE ISC]].
     exists n'; auto. }
-  { specialize (IHEV st' eq_refl). good_inversion ISC_NEXT.
+  { specialize (IHEV nst' eq_refl). good_inversion ISC_NEXT.
     { good_inversion ISC. exists n0.
       eapply counter_in_answer in EV. split; auto. }
     { good_inversion ISC. apply IHEV in ISC0.
@@ -162,17 +193,17 @@ Proof.
 Qed.
 
 Lemma well_formed_subst_in_answer
-      (st' : state')
+      (nst : nt_state)
       (s : subst)
       (n : nat)
       (st : state)
-      (EV : eval_step st' (Answer s n) st)
-      (WF : well_formed_state' st') :
+      (EV : eval_step nst (Answer s n) st)
+      (WF : well_formed_nt_state nst) :
       (forall x, in_subst_dom s x -> x < n) /\ (forall x, in_subst_vran s x -> x < n).
 Proof.
   remember (Answer s n). induction EV; good_inversion Heql; good_inversion WF; auto.
   assert (FV_LT_N_1 : forall x, In x (fv_term (apply_subst s0 t1)) -> x < n).
-  { clear MGU s'. intros. induction t1.
+  { clear MGU. clear d. intros. induction t1.
     { simpl in H. destruct (image s0 n0) eqn:eq; auto.
       apply VRAN_LT_COUNTER. red. eauto. }
     { good_inversion H. }
@@ -184,7 +215,7 @@ Proof.
         good_inversion X_FV; auto. apply fvUnifyL. simpl.
         apply set_union_intro. right. auto. } } }
   assert (FV_LT_N_2 : forall x, In x (fv_term (apply_subst s0 t2)) -> x < n).
-  { clear MGU s'. intros. induction t2.
+  { clear MGU. clear d. intros. induction t2.
     { simpl in H. destruct (image s0 n0) eqn:eq; auto.
       apply VRAN_LT_COUNTER. red. eauto. }
     { good_inversion H. }
@@ -205,18 +236,18 @@ Proof.
 Qed.
 
 Lemma well_formedness_preservation
-      (st' : state')
+      (nst : nt_state)
       (l : label)
       (st : state)
-      (EV : eval_step st' l st)
-      (WF : well_formed_state' st') :
+      (EV : eval_step nst l st)
+      (WF : well_formed_nt_state nst) :
       well_formed_state st.
 Proof.
   intros. induction EV; good_inversion WF; auto.
   { constructor. auto. }
   { constructor. constructor; auto.
     intros. good_inversion FRN_COUNTER. subst. auto. }
-  { constructor. constructor.
+  { constructor. constructor; auto.
     1-2: intros; eapply lt_trans; eauto.
     intros. destruct (eq_nat_dec n x).
     { omega. }
@@ -226,7 +257,7 @@ Proof.
     simpl in CC. destruct CC as [CL _]. red in CL. red in CL. auto. }
   { specialize (IHEV WF_L).
     good_inversion IHEV. auto. }
-  { constructor. constructor.
+  { constructor. constructor; auto.
     1-2: apply well_formed_subst_in_answer in EV; destruct EV; auto.
     intros. apply FV_LT_COUNTER; auto. eapply counter_in_answer; eauto. }
   { specialize (IHEV WF_L). good_inversion IHEV.
@@ -249,90 +280,90 @@ Proof.
 Qed.
 
 Lemma eval_step_exists
-      (st' : state') :
-      {l : label & {st : state & eval_step st' l st}}.
+      (nst : nt_state) :
+      {l : label & {st : state & eval_step nst l st}}.
 Proof.
-  induction st'.
+  induction nst.
   { destruct g.
-    1-2,4-7: repeat eexists; econstructor.
+    1,3-6: repeat eexists; econstructor.
     { assert ({r & mgu (apply_subst s t) (apply_subst s t0) r}).
-      { apply mgu_exists. }
+      { apply mgu_result_exists. }
       destruct H. destruct x.
-      all: repeat eexists; eauto. } }
-  { destruct IHst'1 as [l1 [st1 IH1]]. destruct st1.
+      { repeat eexists; eauto. }
+      { repeat eexists; eauto. } } }
+  { destruct IHnst1 as [l1 [st1 IH1]]. destruct st1.
     all: repeat eexists; eauto. }
-  { destruct IHst' as [l [st IH]]. destruct st; destruct l.
+  { destruct IHnst as [l [st IH]]. destruct st; destruct l.
     all: repeat eexists; eauto. }
-Qed.
+Defined.
 
 Lemma eval_step_unique
-      (st' : state')
+      (nst : nt_state)
       (l1 l2 : label)
       (st1 st2 : state)
-      (STEP_1 : eval_step st' l1 st1)
-      (STEP_2 : eval_step st' l2 st2) :
+      (STEP_1 : eval_step nst l1 st1)
+      (STEP_2 : eval_step nst l2 st2) :
       l1 = l2 /\ st1 = st2.
 Proof.
-  revert STEP_1 STEP_2. revert l1 l2 st1 st2. induction st'.
+  revert STEP_1 STEP_2. revert l1 l2 st1 st2. induction nst.
   { intros. destruct g; good_inversion STEP_1; good_inversion STEP_2; auto.
-    { assert (C : None = Some s').
-      { eapply mgu_unique; eassumption. }
+    { assert (C : None = Some d).
+      { eapply mgu_result_unique; eassumption. }
       inversion C. }
-    { assert (C : None = Some s').
-      { eapply mgu_unique; eassumption. }
+    { assert (C : None = Some d).
+      { eapply mgu_result_unique; eassumption. }
       inversion C. }
-    { assert (C : Some s' = Some s'0).
-      { eapply mgu_unique; eassumption. }
-      inversion C. auto. } }
+    { assert (EQ : Some d = Some d0).
+      { eapply mgu_result_unique; eassumption. }
+      good_inversion EQ. auto. } }
   { intros. good_inversion STEP_1; good_inversion STEP_2;
-    specialize (IHst'1 _ _ _ _ STEP_L STEP_L0); inversion IHst'1;
+    specialize (IHnst1 _ _ _ _ STEP_L STEP_L0); inversion IHnst1;
     inversion H0; subst; auto. }
   { intros. good_inversion STEP_1; good_inversion STEP_2;
-    specialize (IHst' _ _ _ _ STEP_L STEP_L0); inversion IHst'; subst;
+    specialize (IHnst _ _ _ _ STEP_L STEP_L0); inversion IHnst; subst;
     inversion H; inversion H0; auto. }
 Qed.
 
-(* Traces *)
+
+
+(***************** Operational Semantics ******************)
+
 Definition trace : Set := @stream label.
 
 CoInductive op_sem : state -> trace -> Set :=
 | osStop : op_sem Stop Nil
-| osState : forall st' l st t (EV: eval_step st' l st)
-                              (OP: op_sem st t),
-                              op_sem (State st') (Cons l t).
+| osNTState : forall nst l st t (EV: eval_step nst l st)
+                                (OP: op_sem st t),
+                                op_sem (NTState nst) (Cons l t).
 
-Hint Constructors op_sem.
+Hint Constructors op_sem : core.
 
 CoFixpoint trace_from (st : state) : trace :=
   match st with
   | Stop => Nil
-  | State st' =>
-    match eval_step_exists st' with
-    | existT _ l (existT _ st'' ev_st'_st'') =>
-      Cons l (trace_from st'')
+  | NTState nst =>
+    match eval_step_exists nst with
+    | existT _ l (existT _ nst' ev_nst_nst') =>
+      Cons l (trace_from nst')
     end
   end.
 
-Lemma trace_from_correct 
+Lemma trace_from_correct
       (st : state) :
       op_sem st (trace_from st).
 Proof.
   revert st. cofix CIH. destruct st.
   { rewrite helper_eq. simpl. constructor. }
-  { rewrite helper_eq. simpl. destruct (eval_step_exists s).
-    destruct s0. econstructor; eauto. }
-Qed.
+  { rewrite helper_eq. simpl. destruct (eval_step_exists n).
+    destruct s. econstructor; eauto. }
+Defined.
 
 Lemma op_sem_exists
       (st : state) :
       {t : trace & op_sem st t}.
 Proof.
   eexists. eapply trace_from_correct.
-Qed.
-
-Extraction Language Haskell.
-
-Extraction "extracted/interpreter.hs" op_sem_exists.
+Defined.
 
 Lemma op_sem_unique
       (st : state)
@@ -352,24 +383,30 @@ Proof.
     { subst. eapply CIH; eauto. } }
 Qed.
 
+Definition in_denotational_analog (t : trace) (f : repr_fun) : Prop :=
+  exists (s : subst) (n : nat),
+    in_stream (Answer s n) t /\ [ s ,  f ].
+
+Notation "{| t , f |}" := (in_denotational_analog t f).
+
 Lemma counter_in_trace
       (g : goal)
       (s sr : subst)
       (n nr : nat)
       (tr : trace)
-      (OP : op_sem (State (Leaf g s n)) tr)
+      (OP : op_sem (NTState (Leaf g s n)) tr)
       (HIn : in_stream (Answer sr nr) tr) :
       n <= nr.
 Proof.
-  remember (Leaf g s n) as st'.
-  assert (CNT_GE : forall n', is_counter_of_state' n' st' -> n <= n').
+  remember (Leaf g s n) as nst.
+  assert (CNT_GE : forall n', is_counter_of_nt_state n' nst -> n <= n').
   { intros. subst. good_inversion H. auto. }
-  clear Heqst'. revert CNT_GE OP. revert n st'.
+  clear Heqnst. revert CNT_GE OP. revert n nst.
   remember (Answer sr nr). induction HIn; intros; subst.
   { good_inversion OP. apply counter_in_answer in EV. auto. }
   { good_inversion OP. destruct st.
     { good_inversion OP0. good_inversion HIn. }
-    { apply IHHIn with s0; auto. intros.
+    { apply IHHIn with n0; auto. intros.
       specialize (counter_in_next_state _ _ _ _ EV H). intros.
       destruct H0. destruct H0. apply CNT_GE in H1.
       eapply le_trans; eauto. } }
@@ -394,15 +431,16 @@ Proof.
     eapply well_formedness_preservation; eauto. }
 Qed.
 
+
 Lemma sum_op_sem
-      (st'1 st'2 : state')
+      (nst1 nst2 : nt_state)
       (t1 t2 t : trace)
-      (OP_1 : op_sem (State st'1) t1)
-      (OP_2 : op_sem (State st'2) t2)
-      (OP_12 : op_sem (State (Sum st'1 st'2)) t) :
+      (OP_1 : op_sem (NTState nst1) t1)
+      (OP_2 : op_sem (NTState nst2) t2)
+      (OP_12 : op_sem (NTState (Sum nst1 nst2)) t) :
       interleave t1 t2 t.
 Proof.
-  revert OP_1 OP_2 OP_12. revert t1 t2 t st'1 st'2.
+  revert OP_1 OP_2 OP_12. revert t1 t2 t nst1 nst2.
   cofix CIH. intros. inversion OP_1. subst. inversion OP_12. subst.
   inversion EV0; subst; specialize (eval_step_unique _ _ _ _ _ EV STEP_L);
   intros [EQL EQST]; subst; constructor.
@@ -413,56 +451,62 @@ Proof.
   { eapply CIH; eassumption. }
 Qed.
 
-Lemma disjunction_finite_commutativity
+Lemma sum_op_sem_in
+      (nst1 nst2 : nt_state)
+      (t1 t2 t : trace)
+      (r : label)
+      (OP_1 : op_sem (NTState nst1) t1)
+      (OP_2 : op_sem (NTState nst2) t2)
+      (OP_12 : op_sem (NTState (Sum nst1 nst2)) t) :
+      in_stream r t <-> in_stream r t1 \/ in_stream r t2.
+Proof.
+  apply interleave_in. eapply sum_op_sem; eauto.
+Qed.
+
+Lemma disj_termination
       (g1 g2 : goal)
       (s : subst)
       (n : nat)
-      (t12 t21 : trace)
-      (OP_12 : op_sem (State (Leaf (Disj g1 g2) s n)) t12)
-      (OP_21 : op_sem (State (Leaf (Disj g2 g1) s n)) t21)
-      (FIN_12 : finite t12) :
-      finite t21.
+      (t1 t2 t : trace)
+      (r : label)
+      (OP_1 : op_sem (NTState (Leaf g1 s n)) t1)
+      (OP_2 : op_sem (NTState (Leaf g2 s n)) t2)
+      (OP_12 : op_sem (NTState (Leaf (Disj g1 g2) s n)) t) :
+      finite t <-> finite t1 /\ finite t2.
 Proof.
-  intros.
-  inversion OP_12; subst.
-  inversion EV; subst.
-  inversion FIN_12; subst.
-  inversion OP_21; subst.
-  inversion EV0; subst.
-  constructor.
-  specialize (op_sem_exists (State (Leaf g1 s n))). intro. destruct H as [t1 OP1].
-  specialize (op_sem_exists (State (Leaf g2 s n))). intro. destruct H as [t2 OP2].
-  specialize (sum_op_sem _ _ _ _ _ OP1 OP2 OP). intro.
-  specialize (sum_op_sem _ _ _ _ _ OP2 OP1 OP0). intro.
-  specialize (interleave_finite _ _ _ H). intro.
-  specialize (interleave_finite _ _ _ H0). intro.
-  apply H2. apply and_comm. apply H1. auto.
+  good_inversion OP_12. good_inversion EV.
+  assert (forall t, finite (Cons Step t) <-> finite t).
+  { intros; split; intros H.
+    { inversion H; auto. }
+    { constructor; auto. } }
+  eapply RelationClasses.iff_Transitive. eapply (H t0).
+  apply interleave_finite. eapply sum_op_sem; eauto.
 Qed.
 
 Lemma prod_op_sem_in
-      (st' : state')
+      (nst : nt_state)
       (g : goal)
       (s : subst)
       (n : nat)
       (t1 t2 t : trace)
       (r : label)
-      (OP : op_sem (State (Prod st' g)) t)
-      (OP1 : op_sem (State st') t1)
-      (OP2 : op_sem (State (Leaf g s n)) t2)
+      (OP : op_sem (NTState (Prod nst g)) t)
+      (OP1 : op_sem (NTState nst) t1)
+      (OP2 : op_sem (NTState (Leaf g s n)) t2)
       (IN_1 : in_stream (Answer s n) t1)
       (IN_2 : in_stream r t2) :
       in_stream r t.
 Proof.
-  revert OP OP1. revert t st'. remember (Answer s n) as r1.
+  revert OP OP1. revert t nst. remember (Answer s n) as r1.
   induction IN_1; intros; subst.
   { good_inversion OP1. good_inversion OP.
     good_inversion EV0; specialize (eval_step_unique _ _ _ _ _ EV STEP_L);
     intro eqs; destruct eqs; subst; good_inversion H.
     { constructor. specialize (op_sem_unique _ _ _ OP2 OP1).
       intros. eapply in_equal_streams; eauto. }
-    { constructor. specialize (op_sem_exists (State (Leaf g s0 n0))).
+    { constructor. specialize (op_sem_exists (NTState (Leaf g s0 n0))).
       intro H. destruct H as [t3 OP3].
-      specialize (op_sem_exists (State (Prod st'0 g))).
+      specialize (op_sem_exists (NTState (Prod nst' g))).
       intro H. destruct H as [t4 OP4].
       specialize (sum_op_sem _ _ _ _ _ OP3 OP4 OP1).
       intro interH. eapply interleave_in in interH.
@@ -474,11 +518,19 @@ Proof.
     intro eqs; destruct eqs; subst.
     1-2: good_inversion OP0; good_inversion IN_1.
     { constructor. eapply IHIN_1; eauto. }
-    { constructor. specialize (op_sem_exists (State (Leaf g s0 n0))).
+    { constructor. specialize (op_sem_exists (NTState (Leaf g s0 n0))).
       intro H. destruct H as [t3 OP3].
-      specialize (op_sem_exists (State (Prod st'0 g))).
+      specialize (op_sem_exists (NTState (Prod nst' g))).
       intro H. destruct H as [t4 OP4].
       specialize (sum_op_sem _ _ _ _ _ OP3 OP4 OP1).
       intro interH. eapply interleave_in in interH.
       eapply interH. right. eapply IHIN_1; eauto. } }
 Qed.
+
+
+Extraction Language Haskell.
+
+Extraction "/Users/rozplokhas/JB/OCanren/miniKanren-coq-thesis/extracted/interpreter.hs" op_sem_exists.
+
+
+
